fstar/common/code/MLS.NetworkTypes.fst
@@ -134,7 +134,7 @@ type extension_nt (bytes:Type0) {|bytes_like bytes|} = {
 [@@"opaque_to_smt"]
 val ps_option:
   #bytes:Type0 -> {|bytes_like bytes|} -> #a:Type0 ->
-  parser_serializer bytes a ->
+  parser_serializer_prefix bytes a ->
   parser_serializer bytes (option a)
 let ps_option #bytes #bl #a ps_a =
   let n_pred = (fun n -> n <= 1) in
